\documentclass[11pt, A4paper,norsk]{article}
\usepackage[utf8]{inputenc}
\usepackage[T1]{fontenc}
\usepackage{babel}
\usepackage{amsmath}
\usepackage{amsfonts}
\usepackage{amsthm}
\usepackage{amssymb}
\usepackage[colorlinks]{hyperref}
\usepackage{listings}
\usepackage{color}
\usepackage{hyperref}
\usepackage{graphicx}
\usepackage{cite}
\usepackage{textcomp}
\usepackage{float}

\definecolor{dkgreen}{rgb}{0,0.6,0}
\definecolor{gray}{rgb}{0.5,0.5,0.5}
\definecolor{daynineyellow}{rgb}{1.0,0.655,0.102}
\definecolor{url}{rgb}{0.1,0.1,0.4}

\lstset{frame=tb,
	language=Python,
	aboveskip=3mm,
	belowskip=3mm,
	showstringspaces=false,
	columns=flexible,
	basicstyle={\small\ttfamily},
	numbers=none,
	numberstyle=\tiny\color{gray},
	keywordstyle=\color{blue},
	commentstyle=\color{daynineyellow},
	stringstyle=\color{dkgreen},
	breaklines=true,
	breakatwhitespace=true,
	tabsize=3
}

\lstset{inputpath="C:/Users/Torstein/Documents/UiO/Fys3140/Python programmer"}
\graphicspath{{C:/Users/Torstein/Documents/UiO/Fys3140/"Python programmer"/}}
\hypersetup{colorlinks, urlcolor=url}

\author{Torstein Solheim Ølberg}
\title{Svar på Oblig nr. 8 i Fys2140}



%\lstinputlisting{Filnavn! type kodefil}
%\includegraphics[width=12.6cm,height=8cm]{Filnavn! type png}



\begin{document}
\maketitle
	\begin{center}
\Large \textbf{Oppgaver}
	\end{center}









		\paragraph{8.1}
			\begin{flushleft}
Alle ikke-åpenbare integraler er løst ved hjelp av \url{www.wolframalpha.com}
			\end{flushleft}
			\subparagraph{a)}
				\begin{gather*}
dy + (2xy - x e^{- x^2}) dx = 0 \\
e^{x^2} dy + ( 2x e^{x^2}y - x ) dx = 0 \\
\int e^{x^2} dy = e^{x^2}y + C(x) \\
\int 2x e^{x^2} y - x dx = e^{x^2} y + x^2 + D(y) \\
C(x) = x^2 \wedge D(y) = 0 \\
F(x, y) = e^{x^2} y + x^2 = A \\
y = \frac{A - x^2}{e^{x^2}} = A e^{- x^2} - x^2 e^{- x^2}
				\end{gather*}









			\subparagraph{b)}
				\begin{gather*}
y' + y \cos(x) = \sin(2 x) \\
dy + (y \cos(x) - \sin(2 x))dx = 0 \\
e^{\sin(x)} dy + ( \cos(x) e^{\sin(x)} y - \sin(2 x) e^{\sin(x)})dx = 0 \\
\int e^{\sin(x)} dy = e^{\sin(x)} y + C(x) \\
\int \cos(x) e^{\sin(x)} y - \sin(2 x) e^{\sin(x)} dx = e^{\sin(x)} y - 2 e^{\sin(x)} (\sin(x) - 1) + D(y) \\
F(x, y) = e^{\sin(x)} y - 2 e^{\sin(x)} (\sin(x) - 1) = A \\
y = \frac{A + 2 e^{\sin(x)} (\sin(x) - 1)}{e^{\sin(x)}} = A e^{- \sin(x)} + 2 (\sin(x) - 1)
				\end{gather*}









			\subparagraph{c)}
				\begin{gather*}
y' \cos(x) + y = \cos^2(x) \\
dy + (\frac{1}{\cos(x)} y - \cos(x)) dx = 0 \\
e^{\int \frac{1}{\cos(x)} dx} dy + \left( \frac{1}{\cos(x)} e^{\int \frac{1}{\cos(x)} dx} y - \cos(x) e^{\int \frac{1}{\cos(x)} dx} \right) dx = 0 \\
\int \frac{1}{\cos(x)} e^{\int \frac{1}{\cos(x)} dx} y - \cos(x) e^{\int \frac{1}{\cos(x)} dx} dx = e^{\int \frac{1}{\cos(x)} dx} - (x - \cos(x)) \\
F = A = y e^{\ln( \sec(x) + \tan(x) )} - (x - \cos(x)) \\
y = \frac{A + (x - \cos(x))}{e^{\ln( \sec(x) + \tan(x) )}} \\
y = \frac{A + (x - \cos(x))}{\sec(x) + \tan(x)}
				\end{gather*}
			








		\paragraph{8.2}
			\subparagraph{a)}
				\begin{gather*}
4y'' + 12y' + 9 = 0 \\
r = \frac{d}{dx}
r^2 + 3 r + \frac{9}{4} = 0 \\
r = \frac{- 3 \pm \sqrt{3^2 - 4 \cdot 1 \cdot \frac{9}{4}}}{2} = \frac{-3 \pm \sqrt{9 - 9}}{2} = - \frac{3}{2} \\
\left( r + \frac{3}{2} \right)^2y = 0 \\
y = ( A + Bx ) e^{- \frac{3}{2} x}
				\end{gather*}










			\subparagraph{b)}
				\begin{gather*}
y'' - 4y' + 13y = 0 \\
r = \frac{d}{dx} \\
r^2 - 4r + 13 = 0 \\
r = \frac{4 \pm \sqrt{4^2 - 4 \cdot 13}}{2} = \frac{4 \pm 2 \sqrt{-9}}{2} = \frac{4 \pm 2i3}{2} = 2 \pm 3i \\
(r - 2 - 3i)(r - 2 + 3i)y = 0 \\
y =C  e^{2 x} \sin(3 x + D)
				\end{gather*}









		\paragraph{8.3}
			\subparagraph{a)}
				\begin{gather*}
xy'' - 2(x + 1)y' + (x + 2)y = 0 \\
\text{En løsning er $u(x) = e^{x}$} \\
\text{Prøver med løsningen $y = u(x)v(x) = e^{x}v(x)$} \\
y' = v'e^{x} + ve^{x} \wedge y'' = v''e^{x} + 2 v'e^{x} + ve^{x} \\
x\left( v''e^{x} + 2 v'e^{x} + ve^{x} \right) - 2(x + 1) \left( v'e^{x} + ve^{x} \right) + (x + 2) v e^{x} = 0 \\
xv''e^{x} + 2xv'e^{x} + xve^{x} - 2(x + 1)v'e^{x} - 2(x + 1)ve^{x} + (x + 2)ve^{x} = 0 \\
(xe^{x} - 2(x + 1)e^{x} + (x + 2)e^{x})v + (2xe^{x} - 2(x + 1)e^{x})v' + xe^{x}v'' = 0 \\
(2xe^{x} - 2(x + 1)e^{x})v' + xe^{x}v'' = 0 \\
V = v' \\
V' + \frac{(2xe^{x} - 2xe^{x} - 2e^{x})}{xe^{x}}V = V' - \frac{2}{x} V = 0 \\
\frac{dV}{V} = \frac{2}{x} dx \\
\int \frac{dV}{V} = \int \frac{2}{x} dx \\
\ln(V) = 2ln(x) + A \\
V = Bx^2 \\
v = \int Bx^2 dx = B \frac{1}{3} x^3 \\
y = C x^3e^{x}
				\end{gather*}









			\subparagraph{b)}
				\begin{gather*}
x^2 y'' + (x + 1)y' - y = 0 \\
\text{En løsning er $u(x) = x + 1$} \\
\text{Prøver med løsningen $y = u(x)v(x) = v(x)(x + 1)$} \\
y' = v'(x + 1) + v \wedge v''(x + 1) + 2v' \\
x^2 (v''(x + 1) + 2v') + (x + 1)(v'(x + 1) + v) - v(x + 1) = 0 \\
x^2(x + 1) v'' + x^2 2 v' + (x + 1)^2 v' + (x + 1) v - (x + 1)v = 0 \\
x^2(x + 1) v'' + ( 2 x^2 + (x + 1)^2 ) v' + ( (x + 1) - (x + 1) ) v = 0 \\
( x^3 + x^2 ) v'' + ( 3 x^2 + 2x + 1 ) v' = 0 \\
\frac{v''}{v'} = - \frac{3 x^2 + 2x + 1}{x^3 + x^2}
V = v' \\
\frac{V'}{V} = - \frac{3 x^2 + 2x + 1}{x^3 + x^2} \\
\frac{dV}{V} = - \frac{3 x^2 + 2x + 1}{x^3 + x^2} dx \\
\int \frac{dV}{V} = \int - \frac{3 x^2 + 2x + 1}{x^3 + x^2} dx \\
\ln(V) = \frac{1}{x} - ln(x) - 2ln(x + 1) + A \\
V = e^{\frac{1}{x} - ln(x) - 2ln(x + 1) + A} \\
V = e^{\frac{1}{x}} \frac{1}{x} \frac{1}{(x + 1)^2} e^{A} \\
V = \frac{B e^{\frac{1}{x}}}{x^3 + 2x^2 + x} \\
v = \int V dx = \int \frac{B e^{\frac{1}{x}}}{x^3 + 2x^2 + x} dx = C \frac{x e^{\frac{1}{x}}}{x + 1} \\
y = (x + 1) C \frac{x e^{\frac{1}{x}}}{x + 1} = C x e^{\frac{1}{x}}
				\end{gather*}
\end{document}